exploring inducting on the compilation funciton

Hs/Algorithm.lean
@@ -2,78 +2,83 @@ import Hs.HsJudgment
 import Hs.HsTerm
 import SystemFD.Term
 
-def compile (Γ : Ctx HsTerm) (t : HsTerm) (τ : HsTerm) : Γ ⊢s t : τ -> Option Term
+def compile_kind (Γ : Ctx HsTerm) (κ : HsTerm) (ty : HsTerm) : Γ ⊢κ κ : ty -> Option Term
+| .ax _ => some ★
+| @HsJudgment.arrowk Γ A B j1 j2 => do
+  let t1 <- compile_kind Γ A `□ j1
+  let t2 <- compile_kind Γ B `□ j2
+  .some (t1 -k> t2)
+
+def compile_type (Γ : Ctx HsTerm) (τ : HsTerm) (k : HsTerm) : Γ ⊢τ τ : k -> Option Term
 -----------------------------
 ----- Types and kinds
 -----------------------------
-| .ax _ => some ★
-| @HsJudgment.arrowk Γ A B j1 j2 => do
-  let t1 <- compile Γ A `□ j1
-  let t2 <- compile Γ B `□ j2
-  .some (t1 -k> t2)
+| @HsJudgment.varTy _ x _ _ _ _ => .some #x
 | @HsJudgment.appk Γ f A B a j1 j2 => do
-  let t1 <- compile Γ f (A `-k> B) j1
-  let t2 <- compile Γ a A j2
+  let t1 <- compile_type Γ f (A `-k> B) j1
+  let t2 <- compile_type Γ a A j2
   .some (t1 `@k t2)
 | @HsJudgment.allt Γ A B j1 j2 => do
-  let t1 <- compile Γ A `□ j1
-  let t2 <- compile (.kind A :: Γ) B `★ j2
+  let t1 <- compile_kind Γ A `□ j1
+  let t2 <- compile_type (.kind A :: Γ) B `★ j2
   .some (∀[t1] t2)
-| @HsJudgment.arrow Γ A B j1 j2 => do
-  let t1 <- compile Γ A `★ j1
-  let t2 <- compile (.empty ::Γ) B `★ j2
+| @HsJudgment.arrow Γ A B j1 _ j2 => do
+  let t1 <- compile_type Γ A `★ j1
+  let t2 <- compile_type (.empty ::Γ) B `★ j2
   .some (t1 -t> t2)
 | @HsJudgment.farrow Γ A B j1 _ j2 => do
-  let t1 <- compile Γ A `★ j1
-  let t2 <- compile (.empty ::Γ) B `★ j2
+  let t1 <- compile_type Γ A `★ j1
+  let t2 <- compile_type (.empty ::Γ) B `★ j2
   .some (t1 -t> t2)
 
+
+def compile_term (Γ : Ctx HsTerm) (t : HsTerm) (τ : HsTerm) : Γ ⊢t t : τ -> Option Term
 --------------------------------------------
 ----- terms
 -----------------------------------------
-| @HsJudgment.var _ x _ _ _ => #x
+| @HsJudgment.var _ x _ _ _ _ => #x
 | @HsJudgment.lam Γ A t B j1 j2 _ => do
-  let A' <- compile Γ A `★ j1
-  let t' <- compile (.type A :: Γ) t B j2
+  let A' <- compile_type Γ A `★ j1
+  let t' <- compile_term (.type A :: Γ) t B j2
   .some (`λ[A'] t')
 | @HsJudgment.app Γ t1 A B t2 B' j1 j2 _ => do
-  let t1' <- compile Γ t1 (A → B) j1
-  let t2' <- compile Γ t2 A j2
+  let t1' <- compile_term Γ t1 (A → B) j1
+  let t2' <- compile_term Γ t2 A j2
   .some (t1' `@ t2')
 | @HsJudgment.hslet Γ A t1 t2 B j1 j2 j3 j4 => do
-  let A' <- compile Γ  A `★ j1
-  let t1' <- compile Γ t1 A j2
-  let t2' <- compile (.term A t1 :: Γ) t2 ([S]B) j3
+  let A' <- compile_type Γ  A `★ j1
+  let t1' <- compile_term Γ t1 A j2
+  let t2' <- compile_term (.term A t1 :: Γ) t2 ([S]B) j3
   .some (.letterm A' t1' t2')
 | @HsJudgment.hsIte Γ p A s R i B t T j1 j2 j3 j4 _ _ _ _ _ _  => do
-  let p' <- compile Γ p A j1
-  let s' <- compile Γ s R j2
-  let i' <- compile Γ i B j3
-  let t' <- compile Γ t T j4
+  let p' <- compile_term Γ p A j1
+  let s' <- compile_term Γ s R j2
+  let i' <- compile_term Γ i B j3
+  let t' <- compile_term Γ t T j4
   .some (.ite p' s' i' t')
 
 ----------------------------------------
 --- Implicit
 ----------------------------------------
 | @HsJudgment.implicitAllE Γ t A τ e j1 j2  => do
-  let t1 <- (compile Γ t (`∀{A}τ) j1)
-  let t2 <- (compile Γ e A j2)
+  let t1 <- (compile_term Γ t (`∀{A}τ) j1)
+  let t2 <- (compile_term Γ e A j2)
   .some (t1 `@t t2)
 | @HsJudgment.implicitAllI Γ A t τ j1 j2 j3 => do
-  let t' <- compile (.kind A :: Γ) t τ j1
-  let A' <- compile Γ A `□ j2
+  let t' <- compile_term (.kind A :: Γ) t τ j1
+  let A' <- compile_kind Γ A `□ j2
   .some (Λ[A']t')
 | @HsJudgment.implicitArrI Γ π τ t j1 j2 _ j3 => do
-  let π' <- compile Γ π `★ j1
-  let t' <- compile (.type π :: Γ) t τ j3
+  let π' <- compile_type Γ π `★ j1
+  let t' <- compile_term (.type π :: Γ) t τ j3
   .some (`λ[π'] t')
 | @HsJudgment.implicitArrE Γ t π τ e j1 j2 => do
-  let t' <- compile Γ t (π ⇒ τ) j1
-  let e' <- compile Γ e π j2
+  let t' <- compile_term Γ t (π ⇒ τ) j1
+  let e' <- compile_term Γ e π j2
   .some (t' `@ e')
 termination_by h => h.size
 
-notation "⟨" t "," τ ";" j "⟩" => Sigma.mk (t, τ) j
+-- notation "⟨" t "," τ ";" j "⟩" => Sigma.mk (t, τ) j
 
 -- def compile_ctx : Ctx (HsTerm, ⟨t, τ; j⟩) -> Option (Ctx Term)
 -- | [] => .some []
