Hs/Metatheory/Preservation2.lean
@@ -1,6 +1,5 @@
 import Hs.Algorithm
 
-
 inductive HsKindLike : HsTerm -> Prop where
 | HsType : HsKindLike `★
 | HsArrK : HsKindLike k -> HsKindLike k' -> HsKindLike (k `-k> k')
@@ -12,21 +11,37 @@ inductive CompileCtx : Ctx HsTerm -> Ctx Term -> Prop where
   CompileCtx (.empty :: Γ) (.empty :: Γ')
 | kind :
   CompileCtx Γ Γ' ->
-  (j1 : Γ ⊢s A : `□) ->
-  compile Γ A `□ j1 = .some A' ->
+  (j1 : Γ ⊢κ A : `□) ->
+  compile_kind Γ A `□ j1 = .some A' ->
   CompileCtx (.kind A :: Γ) (.kind A' :: Γ')
 | type :
   CompileCtx Γ Γ' ->
-  (j1 : Γ ⊢s A : `★) ->
-  compile Γ A `★ j1 = .some A' ->
+  (j1 : Γ ⊢τ A : `★) ->
+  compile_type Γ A `★ j1 = .some A' ->
   CompileCtx (.type A :: Γ) (.type A' :: Γ')
 | term :
   CompileCtx Γ Γ' ->
-  (j1 : Γ ⊢s A : `★)  ->
-  (j2 : Γ ⊢s t : τ) ->
-  compile Γ A `★ j = .some A' ->
-  compile Γ t τ j2 = .some t' ->
+  (j1 : Γ ⊢τ A : `★)  ->
+  (j2 : Γ ⊢t t : τ) ->
+  compile_type Γ A `★ j = .some A' ->
+  compile_term Γ t τ j2 = .some t' ->
   CompileCtx (.term A t :: Γ) (.term A' t' :: Γ')
+
+theorem compile_preserves_indices :
+  CompileCtx Γ Γ' ->
+  (j2 : Γ ⊢κ  T : `□) ->
+  (j1 : Γ ⊢τ `#x : T) ->
+  compile_kind Γ T `□ j = .some T' ->
+  (Γ' d@ x).get_type = .some T' := by
+intro cc j1 j2 ct;
+cases j2;
+induction cc;
+case _ wf h gt => unfold Frame.get_type at gt; simp at gt;
+case _ wf h gt => sorry
+case _ => sorry
+case _ => sorry
+case _ => sorry
+
 
 
 theorem compile_ctx_wf :
@@ -49,35 +64,35 @@ case _ => sorry
 
 theorem kinding_uniqueness :
   HsKindLike τ ->
-  Γ ⊢s τ : k ->
-  Γ ⊢s τ : k' ->
+  Γ ⊢κ τ : k ->
+  Γ ⊢κ τ : k' ->
   k = k' :=
  by
 intro h j1 j2
 induction τ generalizing Γ k k'
 all_goals (cases h)
-case _ => sorry
+case _ => cases j1; cases j2; rfl
 case _ ih1 ih2 kl1 kl2 =>
-  have lem1 := @ih1 Γ `□ `□ kl1;
-  sorry
+  cases j1; cases j2; rfl;
 
 theorem compile_preserves_kinds :
   HsKindLike t ->
   τ = `□ ->
-  (j : Γ ⊢s t : τ) ->
-  compile Γ t τ j = .some t' ->
+  (j : Γ ⊢κ t : τ) ->
+  compile_kind Γ t τ j = .some t' ->
   CompileCtx Γ Γ' ->
   Γ' ⊢ t' : .kind := by
  intro h e j c cc;
- induction Γ, t, τ, j using compile.induct generalizing t'
+ induction Γ, t, τ, j using compile_kind.induct generalizing t'
  all_goals try (cases e)
  all_goals try (cases h)
  case _ =>
-   unfold compile at c; cases c;
-   apply Judgment.ax;
-   sorry
+   unfold compile_kind at c; cases c;
+   case _ wf =>
+     apply Judgment.ax;
+     apply compile_ctx_wf wf cc
  case _ j1 j2 ih1 ih2 kl1 kl2 =>
-   unfold compile at c; simp at c;
+   unfold compile_kind at c; simp at c;
    rw[Option.bind_eq_some] at c;
    cases c; case _ w1 c1 =>
    cases c1; case _ c1 c2 =>
@@ -90,22 +105,146 @@ theorem compile_preserves_kinds :
    apply Judgment.allk;
    apply ih1';
    apply ih2'
--- bogus cases
- case _ j1 ih1 =>  sorry
- case _ => sorry
- case _ => sorry
- case _ => sorry
+
+inductive HsTypeLike : Ctx HsTerm -> HsTerm -> Prop where
+| HsArr : HsTypeLike Γ τ -> HsTypeLike (.empty::Γ) τ' -> HsTypeLike Γ (τ → τ')
+| HsFArr : HsTypeLike Γ τ -> HsTypeLike (.empty::Γ) τ' -> HsTypeLike Γ (τ ⇒ τ')
+| HsVarTy : (Γ d@x).is_datatype || (Γ d@ x).is_kind -> HsTypeLike Γ (`#x)
+| HsAll : HsKindLike A -> HsTypeLike (.kind A::Γ) τ -> HsTypeLike Γ (`∀{A} τ)
+
+theorem typing_uniqueness :
+  HsTypeLike Γ t ->
+  Γ ⊢τ t : k ->
+  Γ ⊢τ t : k' ->
+  k = k' := by
+intro h j1 j2;
+induction t generalizing Γ;
+all_goals (cases h)
+case _ =>
+  cases j1; cases j2
+  case _ h2 _ _ h1 =>
+  rw [<-h1] at h2; injection h2;
+case _ =>
+  cases j1; cases j2;
+  case _ tl1 _ j1 _ _ j2 _ _ ih1 _ =>
+  apply ih1 tl1 j1 j2
+case _ =>
+  cases j1; cases j2;
+  case _ tl1 _ j1 _ _ j2 _ _ ih1 _ =>
+  apply ih1 tl1 j1 j2
+case _ =>
+  cases j1; cases j2;
+  case _ j2 _ _ _ j1 _ ih =>
+  apply ih j2 j1 j1
+
+theorem compile_preserves_types :
+  HsKindLike k ->
+  (j2 : Γ ⊢κ k : `□) ->
+  compile_kind Γ k `□ j2 = .some k' ->
+  HsTypeLike Γ τ ->
+  (j1 : Γ ⊢τ τ : k) ->
+  compile_type Γ τ k j1 = .some τ' ->
+  CompileCtx Γ Γ' ->
+  Γ' ⊢ τ' : k' := by
+intro kl j1 c1 tl j2 c2 cc;
+induction Γ, τ, k, j2 using compile_type.induct generalizing Γ' τ' k'
+all_goals (unfold compile_type at c2; simp at c2)
+case _ =>
+  cases c2;
+  apply Judgment.var;
+  apply compile_ctx_wf; assumption; assumption;
+  sorry
+case _ h1 h2 ih1 ih2 => cases tl
+case _ h1 h2 ih1 =>
+  rw[Option.bind_eq_some] at c2;
+  cases c2; case _ w1 c2 =>
+  cases c2; case _ c2 c3 =>
+  rw[Option.bind_eq_some] at c3;
+  cases c3; case _ w2 c3 =>
+  cases c3; case _ c3 e =>
+  cases e; unfold compile_kind at c1; cases j1;
+  simp at c1; cases c1;
+  cases tl; case _ kl1 kl2 =>
+  apply Judgment.allt;
+  apply compile_preserves_kinds kl1 rfl h1 c2 cc;
+  apply @ih1 ★ w2 (.kind w1 :: Γ') .HsType _ _ kl2 c3 _
+  case _ => apply HsJudgment.ax; apply HsJudgment.wfkind; assumption; assumption
+  case _ => unfold compile_kind; rfl
+  case _ => apply CompileCtx.kind; assumption; assumption
+case _ j1 _ j2 ih1 ih2 =>
+  rw[Option.bind_eq_some] at c2;
+  cases c2; case _ w1 c2 =>
+  cases c2; case _ c2 c3 =>
+  rw[Option.bind_eq_some] at c3;
+  cases c3; case _ w2 c3 =>
+  cases c3; case _ c3 e =>
+  cases e; cases tl;
+  have lem1 := compile_preserves_kinds kl rfl j1 c1 cc;
+  unfold compile_kind at c1; simp at c1;
+  cases j1; simp at c1; cases c1;
+  case _ tl1 tl2 _ =>
+  apply Judgment.arrow;
+  apply @ih1 ★ w1 Γ' .HsType _ _ tl1 c2 cc;
+  case _ => apply HsJudgment.ax; assumption
+  case _ => unfold compile_kind; rfl
+  apply @ih2 ★ w2 (.empty::Γ') .HsType _ _ tl2 c3 _
+  case _ => apply HsJudgment.ax; apply HsJudgment.wfempty; assumption
+  case _ => unfold compile_kind; rfl
+  case _ => apply CompileCtx.empty; assumption
+case _ j1 _ j2 ih1 ih2 =>
+  rw[Option.bind_eq_some] at c2;
+  cases c2; case _ w1 c2 =>
+  cases c2; case _ c2 c3 =>
+  rw[Option.bind_eq_some] at c3;
+  cases c3; case _ w2 c3 =>
+  cases c3; case _ c3 e =>
+  cases e; cases tl;
+  have lem1 := compile_preserves_kinds kl rfl j1 c1 cc;
+  unfold compile_kind at c1; simp at c1;
+  cases j1; simp at c1; cases c1;
+  case _ tl1 tl2 _ =>
+  apply Judgment.arrow;
+  apply @ih1 ★ w1 Γ' .HsType _ _ tl1 c2 cc;
+  case _ => apply HsJudgment.ax; assumption
+  case _ => unfold compile_kind; rfl
+  apply @ih2 ★ w2 (.empty::Γ') .HsType _ _ tl2 c3 _
+  case _ => apply HsJudgment.ax; apply HsJudgment.wfempty; assumption
+  case _ => unfold compile_kind; rfl
+  case _ => apply CompileCtx.empty; assumption
+
+inductive HsTermLike : Ctx HsTerm -> HsTerm -> Prop where
+| HsVar : (Γ d@ x).is_ctor || (Γ d@ x).is_type -> HsTermLike Γ `#x
+| HsApp : HsTermLike Γ t1 -> HsTermLike Γ t2 -> HsTermLike Γ (t1 `• t2)
+| HsLam : HsTermLike (.type A :: Γ) t1 -> HsTermLike Γ (`λ{A}t1)
+| HsIte : HsTermLike Γ p -> HsTermLike Γ i -> HsTermLike Γ t -> HsTermLike Γ e -> HsTermLike Γ (.HsIte p i t e)
+| HsLet : HsTypeLike Γ A -> HsTermLike Γ t -> HsTermLike (.term A t :: Γ) t' -> HsTermLike Γ (.HsLet A t t')
 
 
+theorem compile_preserves_typing :
+  CompileCtx Γ Γ' ->
+  HsTypeLike Γ τ ->
+  (j1 : Γ ⊢τ τ : k) ->
+  compile_type Γ τ k j1 = .some τ' ->
+  HsTermLike Γ t ->
+  (j2 : Γ ⊢t t : τ) ->
+  compile_term Γ t τ j2 = .some t' ->
+  Γ' ⊢ t' : τ' := by
+intro cc τl j1 c1 tl j2 c2;
+induction Γ, t, τ, j2 using compile_term.induct generalizing Γ' t' τ' k
+cases tl;
+all_goals (unfold compile_term at c2; simp at c2)
+case _ => cases c2; sorry
+case _ =>
+ sorry
+case _ =>
+ sorry
+case _ =>
+ sorry
+case _ =>
+ sorry
 
-def is_type : Ctx HsTerm -> HsTerm -> Option Unit
-| Γ, .HsBind2 .arrow k k' => do
-  let _ <- is_type Γ k
-  let _ <- is_type (.empty :: Γ) k'
-  .some ()
-| Γ, .HsBind2 .farrow k k' => do
-  let _ <- is_type Γ k
-  let _ <- is_type (.empty :: Γ) k'
-  .some ()
-| Γ, `#x => if (Γ d@x).is_datatype then .some () else .none
-| _, _ => .none
+-- implicits
+case _ => sorry
+case _ => sorry
+case _ => sorry
+case _ => sorry
