Hs/Example.lean
@@ -5,53 +5,62 @@ import SystemFD.Algorithm
 def idHsTerm : HsTerm := `λ{`#0} `#0
 def idHsType : HsTerm := `∀{`★} `#0 → `#1
 
-def idTypeKinding : [] ⊢s idHsType : `★ := by
+def idTypeKinding : [] ⊢τ idHsType : `★ := by
   unfold idHsType;
   apply HsJudgment.allt;
   case _ => apply HsJudgment.ax (HsJudgment.wfnil)
   case _ =>
     apply HsJudgment.arrow;
     case _ =>
-      apply HsJudgment.var; apply HsJudgment.wfkind; apply HsJudgment.ax (HsJudgment.wfnil);
-      apply HsJudgment.wfnil; unfold Frame.get_type; unfold dnth; unfold Frame.apply; simp;
+      apply HsJudgment.varTy; apply HsJudgment.wfkind; apply HsJudgment.ax (HsJudgment.wfnil);
+      apply HsJudgment.wfnil; simp; unfold Frame.is_datatype; unfold Frame.apply; simp;
+      unfold Frame.is_kind; simp; unfold Frame.get_type; unfold dnth; unfold Frame.apply; simp;
     case _ =>
-      apply HsJudgment.var;
+      apply HsJudgment.varTy;
       apply HsJudgment.wfempty; apply HsJudgment.wfkind; apply HsJudgment.ax (HsJudgment.wfnil);
       apply HsJudgment.wfnil;
-      unfold Frame.get_type; unfold dnth; unfold Frame.apply; simp; unfold Frame.apply; simp
+      simp; unfold Frame.is_kind; unfold Frame.apply; simp; unfold Frame.get_type; unfold dnth;
+      unfold dnth; unfold Frame.apply; simp
 
-def idTyping : [] ⊢s idHsTerm : idHsType := by
+def idTyping : [] ⊢t idHsTerm : idHsType := by
  unfold idHsTerm; unfold idHsType;
  apply HsJudgment.implicitAllI;
  apply HsJudgment.lam;
-   apply HsJudgment.var; apply HsJudgment.wfkind; apply HsJudgment.ax (HsJudgment.wfnil);
-   apply HsJudgment.wfnil; unfold Frame.get_type; unfold dnth; unfold Frame.apply; simp;
+   apply HsJudgment.varTy; apply HsJudgment.wfkind; apply HsJudgment.ax (HsJudgment.wfnil);
+   apply HsJudgment.wfnil; unfold Frame.is_kind; unfold dnth; unfold Frame.apply; simp;
+   unfold Frame.get_type; unfold dnth; unfold Frame.apply; simp;
    apply HsJudgment.var;
-     apply HsJudgment.wftype; apply HsJudgment.var;
-     apply HsJudgment.wfkind; apply HsJudgment.ax (HsJudgment.wfnil);
-       apply HsJudgment.wfnil;
-       unfold Frame.get_type; unfold dnth; unfold Frame.apply; simp;
-       apply HsJudgment.wfkind; apply HsJudgment.ax (HsJudgment.wfnil);
-       apply HsJudgment.wfnil;
-     unfold Frame.get_type; unfold dnth; unfold Frame.apply; simp;
-   case _ =>
-     apply HsJudgment.arrow;
-     apply HsJudgment.var;
-     apply HsJudgment.wfkind; apply HsJudgment.ax (HsJudgment.wfnil); apply HsJudgment.wfnil;
-     unfold Frame.get_type; unfold dnth; unfold Frame.apply; simp;
-     apply HsJudgment.var; apply HsJudgment.wfempty; apply HsJudgment.wfkind;
-     apply HsJudgment.ax (HsJudgment.wfnil); apply HsJudgment.wfnil;
-     unfold Frame.get_type; unfold dnth; unfold Frame.apply; simp; unfold Frame.apply; simp
- apply HsJudgment.ax (HsJudgment.wfnil);
- apply HsJudgment.arrow; apply HsJudgment.var;
+   apply HsJudgment.wftype; apply HsJudgment.varTy;
    apply HsJudgment.wfkind; apply HsJudgment.ax (HsJudgment.wfnil); apply HsJudgment.wfnil;
-   unfold Frame.get_type; unfold dnth; unfold Frame.apply; simp
- apply HsJudgment.var;
- apply HsJudgment.wfempty; apply HsJudgment.wfkind; apply HsJudgment.ax (HsJudgment.wfnil); apply HsJudgment.wfnil;
- unfold Frame.get_type; simp; unfold Frame.apply; simp
+   unfold Frame.is_kind; unfold dnth; unfold Frame.apply; simp;
+   unfold Frame.get_type; unfold dnth; unfold Frame.apply; simp;
+   apply HsJudgment.wfkind; apply HsJudgment.ax (HsJudgment.wfnil);
+   apply HsJudgment.wfnil; unfold Frame.is_type; unfold dnth; unfold Frame.apply; simp;
+   unfold Frame.get_type; unfold dnth; unfold Frame.apply; simp;
+   apply HsJudgment.arrow;
+   apply HsJudgment.varTy;
+   apply HsJudgment.wfkind; apply HsJudgment.ax (HsJudgment.wfnil); apply HsJudgment.wfnil;
+   unfold Frame.is_kind; unfold dnth; unfold Frame.apply; simp;
+   unfold Frame.get_type; unfold dnth; unfold Frame.apply; simp;
+   apply HsJudgment.varTy;
+   apply HsJudgment.wfempty;
+   apply HsJudgment.wfkind; apply HsJudgment.ax (HsJudgment.wfnil); apply HsJudgment.wfnil;
+   unfold Frame.is_kind; unfold dnth; unfold Frame.apply; simp; unfold Frame.apply; simp;
+   unfold Frame.get_type; unfold dnth; unfold Frame.apply; unfold dnth; simp; unfold Frame.apply; simp;
+   apply HsJudgment.ax (HsJudgment.wfnil);
+   apply HsJudgment.arrow;
+   apply HsJudgment.varTy;
+      apply HsJudgment.wfkind; apply HsJudgment.ax (HsJudgment.wfnil); apply HsJudgment.wfnil;
+      unfold Frame.is_kind; unfold dnth; unfold Frame.apply; simp;
+      unfold Frame.get_type; unfold dnth; unfold Frame.apply; simp;
+   apply HsJudgment.varTy;
+      apply HsJudgment.wfempty; apply HsJudgment.wfkind; apply HsJudgment.ax (HsJudgment.wfnil);
+      apply HsJudgment.wfnil;
+      unfold Frame.is_kind; unfold dnth; unfold Frame.apply; simp; unfold Frame.apply; simp;
+      unfold Frame.get_type; unfold dnth; unfold Frame.apply; simp; unfold Frame.apply; simp;
 
-def idType := compile [] idHsType `★ idTypeKinding
-def idTerm := compile [] idHsTerm idHsType idTyping
+def idType := compile_type [] idHsType `★ idTypeKinding
+def idTerm := compile_term [] idHsTerm idHsType idTyping
 
 #guard idType == .some (∀[★] #0 -t> #1)
 #guard idTerm == .some (Λ[★]`λ[#0] #0)
