SystemFD/Algorithm/Completeness1.lean
@@ -1,0 +1,62 @@
+import SystemFD.Term
+import SystemFD.Judgment
+import SystemFD.Ctx
+import SystemFD.Algorithm
+import SystemFD.Metatheory.Classification
+
+set_option maxHeartbeats 500000
+
+@[simp]
+abbrev WfKindCompleteType : (v : JudgmentVariant) -> Ctx Term -> JudgmentArgs v -> Prop
+| .prf => λ Γ => λ (t, τ) => τ = .kind -> Γ = [] -> Γ ⊢ t : τ -> wf_kind t = .some ()
+| .wf  => λ _ => λ () => true
+
+
+theorem wf_kind_complete :
+  ⊢ Γ ->
+  Judgment v Γ idx ->
+  WfKindCompleteType v Γ idx
+:= by
+intros wf j; induction j <;> simp at *;
+case _ =>
+  intro e1 e2 h; subst e1; subst e2
+  cases h; case _ h _ => cases h
+case _ gt _ =>
+  intro e1 e2 h; subst e1; subst e2;
+  case _ =>
+  cases gt;
+case _ h1 h2 ih1 ih2 =>
+  intro e2 h; subst e2;
+  rw[Option.bind_eq_some]; exists ();
+  replace ih1 := ih1 wf rfl h1
+  replace ih2 := ih2 wf rfl h2
+  apply And.intro;
+  assumption
+  rw[Option.bind_eq_some]; exists ();
+case _ =>
+  intro e; subst e;
+  case _ j =>
+  have lem := classification_lemma j; simp at lem;
+  cases lem;
+  case _ h => cases h; case _ h => cases h
+  case _ h =>
+    cases h; case _ w h =>
+    cases h; case _ w1 h =>
+    cases h; cases w1
+case _ =>
+  intro e1 e2; subst e1; subst e2
+  intro h;
+  cases h; case _ h _ => cases h;
+case _ =>
+  intro e h; subst e;
+  cases h; case _ h => cases h;
+all_goals (
+  intro e1 e2 h; subst e1; subst e2;
+  cases h;
+)
+case _ h =>
+  sorry
+case _ h =>
+  sorry
+case _ h =>
+  sorry
